policy_proof/coq/query.v
@@ -1,7 +1,6 @@
 Require Import String.
 
 Require Import types.
-Require Import policy.
 
 Inductive Query: Type :=
   (* Relation *)
@@ -14,5 +13,4 @@ Inductive Query: Type :=
   | QueryGroupBy : Query -> Query -> Query
   (* Selection *).
 
-(* TODO: The third one should be the operator. *)
-Definition config:= (label_lookup, privacy, unit)%type.
+
